src/program_proof/pav/history.v
@@ -6,29 +6,47 @@ From Perennial.program_proof.pav Require Import client core.
 Section defs.
 Context `{!heapGS Σ, !pavG Σ}.
 
-(* TODO: maybe only cliG version needed. not pure or adtrG. *)
+Definition lat_pk_comm_reln (lat_pk : lat_val_ty) (lat_comm : lat_opaque_val_ty) : iProp Σ :=
+  match lat_pk, lat_comm with
+  | Some (ep0, pk), Some (ep1, comm) => ⌜ ep0 = ep1 ⌝ ∗ is_comm pk comm
+  | None, None => True
+  | _, _ => False
+  end.
+
+Definition msv_final (adtr_γ : gname) (ep uid : w64) (lat : lat_val_ty) : iProp Σ :=
+  ∃ (m : adtr_map_ty) (vals : list opaque_map_val_ty),
+  "#Hcomm_reln" ∷ lat_pk_comm_reln lat (last vals) ∗
+  "#Hmap" ∷ mono_list_idx_own adtr_γ (uint.nat ep) m ∗
+  "#Hhist" ∷ ([∗ list] ver ↦ val ∈ vals,
+    ∃ label,
+    "#His_label" ∷ is_vrf uid (W64 ver) label ∗
+    "%Hin_map" ∷ ⌜ m !! label = Some val ⌝) ∗
+  "#Hbound" ∷
+    (∃ label,
+    "#His_label" ∷ is_vrf uid (W64 $ length vals) label ∗
+    "%Hnin_map" ∷ ⌜ m !! label = None ⌝).
+
 Definition know_hist_val_cliG cli_γ (uid ep : w64) (lat : lat_val_ty) : iProp Σ :=
-  ∃ vals,
+  ∃ (vals : list opaque_map_val_ty),
   "%Hbound_vals" ∷ ⌜ length vals < 2^64 ⌝ ∗
-  "%Hlook_lat" ∷ ⌜ last vals = lat ⌝ ∗
+  "#Hcomm_reln" ∷ lat_pk_comm_reln lat (last vals) ∗
   (* prior vers exist in prior or this map. *)
-  "#Hhist" ∷ ([∗ list] ver ↦ '(prior, pk) ∈ vals,
-    (∃ dig m_γ comm,
+  "#Hhist" ∷ ([∗ list] ver ↦ '(prior, comm) ∈ vals,
+    (∃ dig m_γ,
     "%Hlt_prior" ∷ ⌜ uint.Z prior ≤ uint.Z ep ⌝ ∗
     "#Hsubmap" ∷ mono_list_idx_own cli_γ (uint.nat prior) (Some (dig, m_γ)) ∗
-    "#Hin_prior" ∷ (uid, W64 ver) ↪[m_γ]□ Some (prior, comm) ∗
-    "#Hcomm" ∷ is_comm pk comm)) ∗
+    "#Hin_prior" ∷ (uid, W64 ver) ↪[m_γ]□ Some (prior, comm))) ∗
   ( (* next ver doesn't exist in this or later map. *)
     "Hnin_nextver" ∷ (∃ (bound : w64) dig m_γ,
       "%Hgte_bound" ∷ ⌜ uint.Z ep ≤ uint.Z bound ⌝ ∗
       "#Hsubmap" ∷ mono_list_idx_own cli_γ (uint.nat bound) (Some (dig, m_γ)) ∗
-      "#Hin_bound" ∷ (uid, W64 $ length vals) ↪[m_γ] None)
+      "#Hin_bound" ∷ (uid, W64 $ length vals) ↪[m_γ]□ None)
     ∨
     (* next ver exists in later map. *)
     "Hin_nextver" ∷ (∃ (bound : w64) dig m_γ comm,
       "%Hgt_bound" ∷ ⌜ uint.Z ep < uint.Z bound ⌝ ∗
       "#Hsubmap" ∷ mono_list_idx_own cli_γ (uint.nat bound) (Some (dig, m_γ)) ∗
-      "#Hin_bound" ∷ (uid, W64 $ length vals) ↪[m_γ] Some (bound, comm))).
+      "#Hin_bound" ∷ (uid, W64 $ length vals) ↪[m_γ]□ Some (bound, comm))).
 
 Definition get_lat (phys : list map_val_ty) (ep : w64) : lat_val_ty :=
   last $ filter (λ x, uint.Z x.1 ≤ uint.Z ep) phys.
@@ -37,10 +55,10 @@ Definition phys_logic_reln phys (logic : list lat_val_ty) :=
   (∀ (ep : w64) lat, logic !! uint.nat ep = Some lat → lat = get_lat phys ep).
 
 (* know_hist_cliG ties together phys_hist and logic_hist as two different
-hist repr's, either of which may be convenient at any given time. *)
+hist repr's, either of which may be convenient at a given time. *)
 Definition know_hist_cliG cli_γ (uid : w64) (phys_hist : list map_val_ty) (logic_hist : list lat_val_ty) : iProp Σ :=
-  ⌜ phys_logic_reln phys_hist logic_hist ⌝ ∗
-  ([∗ list] ep ↦ lat ∈ logic_hist, know_hist_val_cliG cli_γ uid (W64 ep) lat).
+  "%Hphys_log" ∷ ⌜ phys_logic_reln phys_hist logic_hist ⌝ ∗
+  "#Hknow_vals" ∷ ([∗ list] ep ↦ lat ∈ logic_hist, know_hist_val_cliG cli_γ uid (W64 ep) lat).
 
 Definition own_HistEntry (ptr : loc) (obj : map_val_ty) : iProp Σ :=
   ∃ sl_HistVal,
@@ -53,26 +71,42 @@ Definition own_hist cli_γ uid sl_hist phys_hist : iProp Σ :=
   "Hsl_hist" ∷ own_slice sl_hist ptrT (DfracOwn 1) dim0_hist ∗
   "Hdim0_hist" ∷ ([∗ list] p;o ∈ dim0_hist;phys_hist, own_HistEntry p o) ∗
   "#Hknow_hist" ∷ know_hist_cliG cli_γ uid phys_hist logic_hist.
-
-Definition msv_final (adtr_γ : gname) (ep uid : w64) (lat : lat_val_ty) : iProp Σ.
-Admitted.
 End defs.
 
 Section derived.
 Context `{!heapGS Σ, !pavG Σ}.
 
-Lemma hist_extend_selfmon logic_hist ep cli_γ uid phys_hist :
-  (uint.Z $ length logic_hist) - 1 ≤ uint.nat ep →
+Lemma hist_extend_selfmon logic_hist (ep : w64) cli_γ uid phys_hist :
+  length logic_hist ≤ S $ uint.nat ep →
   ("#Hknow_hist" ∷ know_hist_cliG cli_γ uid phys_hist logic_hist ∗
   "#His_bound" ∷ is_my_bound cli_γ uid (W64 $ length phys_hist) ep) -∗
   ∃ new_hist,
   "%Hlen_hist" ∷ ⌜ length new_hist = S $ uint.nat ep ⌝ ∗
   "Hknow_hist" ∷ know_hist_cliG cli_γ uid phys_hist new_hist.
-Proof. Admitted.
+Proof.
+  intros Hlen_hist. iNamed 1.
+  iExists (logic_hist ++ (replicate ((S $ uint.nat ep) - length logic_hist) (mjoin $ last logic_hist))).
+  iSplit.
+  { iPureIntro. rewrite app_length length_replicate. lia. }
+  iSplit; [admit|].
+  iNamed "Hknow_hist". iFrame "#".
+  iApply big_sepL_forall. iIntros "* %Hlook_repl".
+  apply lookup_replicate in Hlook_repl as [-> ?].
+  destruct (last logic_hist) eqn:Hlook_last; simpl.
+  (* if some last elem, use that for hist. *)
+  - rewrite last_lookup in Hlook_last.
+    iDestruct (big_sepL_lookup with "Hknow_vals") as "Hknow_last"; [exact Hlook_last|].
+    iDestruct "Hknow_last" as (vals) "Hknow_last". iNamed "Hknow_last".
+    iExists vals. iFrame "#%". iSplit.
+    + iApply (big_sepL_impl with "Hhist"). iIntros (?[??]) "!> %". iNamed 1.
+      iFrame "#". iPureIntro. word.
+    + iClear "Hhist Hknow_last". iNamed "His_bound". iLeft. iFrame "#".
+      (* TODO: issue relating length phys_hist with length vals. *)
+Admitted.
 
-Lemma hist_audit_msv ep lat logic_hist aud_ep cli_γ uid phys_hist adtr_γ :
+Lemma hist_audit_msv (ep aud_ep : w64) lat logic_hist cli_γ uid phys_hist adtr_γ :
   logic_hist !! uint.nat ep = Some lat →
-  length logic_hist ≤ aud_ep →
+  Z.of_nat $ length logic_hist ≤ uint.Z aud_ep →
   ("#Hknow_hist" ∷ know_hist_cliG cli_γ uid phys_hist logic_hist ∗
   "#His_audit" ∷ is_audit cli_γ adtr_γ aud_ep) -∗
   "#Hmsv" ∷ msv_final adtr_γ ep uid lat.
